\documentclass[10pt,a4paper]{article}
\usepackage[latin1]{inputenc}
\usepackage{amsmath}
\usepackage{amsfonts}
\usepackage{amssymb}
\usepackage{graphicx}
\author{Carter Rhea}
\title{Homework4}
\begin{document}
	\maketitle
	
	\section{Problem 1}
	Consider the hyperelastic model generated by using the following strain energy density function $\Phi$ :
	$$ \Phi(E) = \lambda \frac{J^2 -1}{4} - (\lambda/2 + \mu)ln(J)+\mu E_{NN} $$

where $\lambda , \mu$ are the Lame parameters (see homework 1), E is the Green strain tensor discussed in class, and J = det F. The trace of E is indicated above by $E_{NN} =E_{11}+E_{22}+E_{33}.$\\
   \textbf{Solution:}\\
   Note: In order to complete this calculation we will need the derivation of $\frac{\partial J}{\partial E_{ij}}$. See appendix for calculation.\\
  
  \begin{equation}
  	\begin{split}
	  \frac{\partial \Phi}{\partial E_{ij}} &= \frac{\partial}{\partial E_{ij}}\Big(\lambda \frac{J^2 -1}{4} - (\lambda/2 + \mu)ln(J)+\mu E_{rs}\delta_{rs}  \Big) \\ 
	    &= \frac{\lambda}{4}*2J\frac{\partial J}{\partial E_{ij}}- (\lambda/2 + \mu)\frac{\frac{\partial J}{\partial{E_{ij}}}}{J}\\
	    &=\frac{\lambda}{2}JJF^{-1}_{Ii}F^{-1}_{Ji}-\frac{\lambda}{2}F^{-1}_{Ii}F^{-1}_{Ji}-\mu F^{-1}_{Ii}F^{-1}_{Ji} + \mu \delta_{IJ}\\
	    &=\mu[\delta_{IJ}-F^{-1}_{Ii}F^{-1}_{Ji}] + \frac{\lambda}{2}(J^2-1)F^{-1}_{Ii}F^{-1}_{Ji}
	\end{split}
  \end{equation}
   
   Now working within indices, show that the material stiffness modulus $C_{IJKL}$ is given given by:
   $$C_{IJKL}:=\frac{\partial S_{IJ}}{\partial E_{KL}} = 2\mu \Big[ 1 + \frac{\lambda}{2\mu}(1-J^2)\Big]F^{-1}_{Im}F^{-1}_{Jn}F^{-1}_{Km}F^{-1}_{Ln}+\lambda J^2 F^{-1}_{Im}F^{-1}_{Jm}F^{-1}_{Kn}F^{-1}_{Ln} $$ 
   
   Note the following relations: \begin{enumerate}
   	\item $$\frac{\partial(F^{-1}_{Ii}F^{-1}_{Ji})}{\partial E_{KL}} = \frac{\partial(F^{-1}F^{-T})_{IJ}}{\partial E_{KL}} $$
    \item $$C = F^TF $$
    \item $$C_{MI}C^{-1}_{IJ} = \delta_{MI}$$
    \item $$C_{MI} = 2E_{MI}-\delta^{MI} $$
    See appendix for calculation of $\frac{\partial C^{-1}_{IJ}}{\partial E_{KL}}$
   \end{enumerate}
   \begin{equation}
   \begin{split}
   C_{IJKL} & =  \mu\frac{\partial \delta_{IJ}}{\partial E_{KL}} -\mu\frac{\partial}{\partial E_{KL}}(F^{-1}_{Ii}F^{-1}_{Ji})  + \frac{\lambda}{2}\frac{\partial}{\partial E_{KL}}\Big[(J^2-1)F^{-1}_{Ii}F^{-1}_{Ji}\Big]\\ 
   & = 2\mu C^{-1}_{IJ}C^{-1}_{KL}+\frac{\lambda}{2}2J^2F^{-1}_{Ki}F^{-1}_{Li}F^{-1}_{I m}F^{-1}_{Jm} + \lambda(J^2-1)C^{-1}_{IJ}C^{-1}_{KL}\\
   & = 2\mu F^{-1}_{Ki}F^{-1}_{Li}F^{-1}_{I m}F^{-1}_{Jm}+\lambda J^2F^{-1}_{Ki}F^{-1}_{Li}F^{-1}_{I m}F^{-1}_{Jm} + \lambda(J^2-1)F^{-1}_{Ki}F^{-1}_{Li}F^{-1}_{I m}F^{-1}_{Jm}\\
   & = 2\mu \Big[ 1 + \frac{\lambda}{2\mu}(1-J^2)\Big]F^{-1}_{Im}F^{-1}_{Jm}F^{-1}_{Ki}F^{-1}_{Li}+\lambda J^2 F^{-1}_{Im}F^{-1}_{Jm}F^{-1}_{Ki}F^{-1}_{Li} 
   \end{split}
   \end{equation}

Show now that $$\sigma_{ij} = \frac{1}{J}F_{iI}S_{IJ}F_{jJ}=\frac{1}{J}\Big[ \mu(F_{iJ}F_{jJ}-\delta_{i}j+\frac{\lambda}{2}(J^2-1)\delta_{ij}) \Big] $$
   
   \begin{equation}
   \begin{split}
    \sigma_{ij} &= \frac{1}{J}F_{iI}S_{IJ}F_{jJ} \\
    & = \frac{1}{J}F_{iI}\Big(\mu[\delta_{IJ}-F^{-1}_{Ii}F^{-1}_{Ji}] + \frac{\lambda}{2}(J^2-1)F^{-1}_{Ii}F^{-1}_{Ji}\Big)F_{jJ}\\
     & = \frac{1}{J}\Big(\mu[F_{iI}\delta_{IJ}F_{jJ}-F_{iI}F^{-1}_{Ii}F^{-1}_{Ji}F_{jJ}] + \frac{\lambda}{2}(J^2-1)F_{iI}F^{-1}_{Ii}F^{-1}_{Ji}F_{jJ}\Big)\\
     & = \frac{1}{J}\Big(\mu[F_{iJ}F_{jJ}-\delta_{ij}] + \frac{\lambda}{2}(J^2-1)\delta)_{ij}\Big)
    \end{split}
   \end{equation}
   And finally show 
   $$c_{ijkl} = \frac{1}{J}F_{iI}F_{jJ}F_{kK}F_{lL}C_{IJKL} = \frac{1}{J} \Big\{ \lambda J^2\delta_{ij}\delta_{kl}+2\mu \Big[ 1+\frac{\lambda}{2\mu}(1-J^2) \Big]d_{ik}d_{kl} \Big\}$$
   
   \begin{equation}
   \begin{split}
   c_{ijkl} &= \frac{1}{J}F_{iI}F_{jJ}F_{kK}F_{lL}C_{IJKL}\\
   &=   \frac{1}{J}F_{iI}F_{jJ}F_{kK}F_{lL}\Big
   \{2\mu \Big[ 1 + \frac{\lambda}{2\mu}(1-J^2)\Big]F^{-1}_{Im}F^{-1}_{Jn}F^{-1}_{Km}F^{-1}_{Ln}+\lambda J^2 F^{-1}_{Im}F^{-1}_{Jm}F^{-1}_{Kn}F^{-1}_{Ln}\Big\}\\
    &=   \frac{1}{J}\Big
   \{2\mu \Big[ 1 + \frac{\lambda}{2\mu}(1-J^2)\Big]F_{iI}F_{jJ}F^{-1}_{Im}F^{-1}_{Jn}F^{-1}_{Km}F^{-1}_{Ln}F_{kK}F_{lL}+\lambda J^2 F_{iI}F_{jJ}F^{-1}_{Im}F^{-1}_{Jm}F^{-1}_{Kn}F^{-1}_{Ln}JF_{kK}F_{lL}\Big\}\\
   &= \frac{1}{J} \Big\{ \lambda J^2\delta_{ij}\delta_{kl}+2\mu \Big[ 1+\frac{\lambda}{2\mu}(1-J^2) \Big]d_{ik}d_{kl} \Big\}
   \end{split}
   \end{equation}
   
   
   If we consider small deformation then $J = 1$ then all the parts where we have $1-J^2 = 0$ 
   
   $$\sigma_{ij} = \frac{1}{J}F_{iI}S_{IJ}F_{jJ}=\frac{1}{J}\Big[ \mu(F_{iJ}F_{jJ}-\delta_{i}j) \Big] $$
   
   $$c_{ijkl} = \frac{1}{J}F_{iI}F_{jJ}F_{kK}F_{lL}C_{IJKL} = \frac{1}{J} \Big\{ \lambda J^2\delta_{ij}\delta_{kl}+2\mu d_{ik}d_{kl} \Big\}$$
   
   
   \section{Appendix}
   \subsection{Derivations}
   \subsubsection{$\frac{\partial J}{\partial E_{ij}}$}
   \begin{equation}
   \begin{split}
      \frac{\partial J}{\partial E_{ij}}  &= \frac{\partial}{\partial E_{ij}} \Big[  (det(2E+I))^{1/2}   \Big] \\ 
      &= \frac{1}{2}(det(2E+I))^{1/2} * cof(2E+I)_{IJ}*2 \\
      &= \frac{1}{J}*det(F^TF)(F^TF)^{-1}_{IJ}\\
      &= JF^{-1}_{Ii}F^{-1}_{Ji}
      \end{split}
   \end{equation}
  
  
   \subsection{$\frac{\partial C^{-1}_{IJ}}{\partial E_{KL}}$}
   \begin{equation}
   \begin{split}
   C_{MI}C^{-1}C_{IJ} = \delta_{MI}\\
	\frac{\partial C_{MI}}{\partial E_{KL}} C^{-1}_{IJ} - C_{MI}\frac{\partial C^{-1}_{IJ}}{\partial E_{KL}} = 0\\
	\frac{\partial(2E_{MI}-\delta_{MI})}{\partial E_{KL}}C^{-1}_{IJ} = C_{MI}\frac{\partial C^{-1}_{IJ}}{\partial E_{KL}}\\
	C^{-1}_{MI}2\frac{\partial E_{MI}}{\partial E_{KL}} = \frac{\partial C^{-1}_{IJ}}{E_{KL}}\\
	2C^{-1}_{MI}\frac{ \delta_{MK} \delta_{IL} \partial E_{KL}}{\partial E_{KL}} = \frac{\partial C^{-1}_{IJ}}{E_{KL}}\\
	 \frac{\partial C^{-1}_{IJ}}{E_{KL}} = 2C^{-1}_{ML}C^{-1}_{IJ}\\
	\end{split}
   \end{equation}












\section{Problem 2}








\end{document}